Here's my thought process for solving the equation x + y / (cosh(x) * sinh(y)) = 0:

1.  **Understand the Goal:** The request is to solve the equation for one variable in terms of the other, or to find specific solutions (x, y).

2.  **Analyze the Equation:** The equation is `x + y / (cosh(x) * sinh(y)) = 0`.
    *   It involves two variables, x and y.
    *   It contains hyperbolic functions: cosh(x) and sinh(y).
    *   There's a division involved, which means we need to consider potential division by zero.

3.  **Identify Potential Issues (Constraints):**
    *   `cosh(x)` is in the denominator. `cosh(x)` is defined as (e^x + e^-x) / 2. This function is always greater than or equal to 1 for real x (cosh(0) = 1). So, `cosh(x)` is never zero for real x. This is good, no constraint on x from this term.
    *   `sinh(y)` is in the denominator. `sinh(y)` is defined as (e^y - e^-y) / 2. This function is zero only when y = 0 (sinh(0) = 0).
    *   Therefore, the equation is *undefined* if `sinh(y) = 0`, which means `y = 0`. We must exclude `y = 0` from any potential solutions derived from the rearranged equation.

4.  **Attempt to Isolate a Variable:**
    *   **Isolating y:** This looks complicated because y appears both linearly (in the numerator) and inside the sinh function (in the denominator). It's unlikely we can get a simple `y = f(x)` form.
    *   **Isolating x:** This also looks complicated because x appears both linearly and inside the cosh function. It's unlikely we can get a simple `x = g(y)` form.

5.  **Rearrange the Equation (Standard Approach):**
    *   Start with `x + y / (cosh(x) * sinh(y)) = 0`.
    *   Subtract x from both sides (assuming `cosh(x) * sinh(y)` is not zero):
        `y / (cosh(x) * sinh(y)) = -x`
    *   Multiply both sides by `cosh(x) * sinh(y)` (again, assuming it's not zero, which means y ≠ 0):
        `y = -x * cosh(x) * sinh(y)`

6.  **Analyze the Rearranged Form:** `y = -x * cosh(x) * sinh(y)`
    *   This is an *implicit* relationship between x and y. It doesn't give an explicit formula for y in terms of x or vice versa.
    *   We still have the constraint `y ≠ 0`.

7.  **Check for Trivial Solutions:**
    *   What if `x = 0`?
        Substitute `x = 0` into the original equation:
        `0 + y / (cosh(0) * sinh(y)) = 0`
        `y / (1 * sinh(y)) = 0`
        `y / sinh(y) = 0`
        This equation requires `y = 0`. However, we already established that `y` cannot be 0 because `sinh(y)` is in the denominator.
        Let's check the rearranged form `y = -x * cosh(x) * sinh(y)`:
        If `x = 0`, we get `y = -0 * cosh(0) * sinh(y)`, which simplifies to `y = 0`.
        So, if we *allow* the limit as y approaches 0, `y/sinh(y)` approaches 1 (since sinh(y) ≈ y for small y). Plugging x=0 into the original equation gives `0 + y/sinh(y) = 0`. In the limit as y->0, this becomes `0 + 1 = 0`, which is false.
        Therefore, `x = 0` does *not* lead to a solution.

    *   What if `y = 0`?
        As established earlier, the original equation is undefined if `y = 0` due to division by `sinh(0) = 0`. So, `y = 0` is not part of any solution.

8.  **Explore Further Rearrangements (less likely to yield explicit solutions but might reveal structure):**
    *   From `y = -x * cosh(x) * sinh(y)`, we could write:
        `y / sinh(y) = -x * cosh(x)`
        This form highlights the structure. The left side depends only on y, and the right side depends only on x. Let `f(y) = y / sinh(y)` and `g(x) = -x * cosh(x)`. We are looking for pairs (x, y) such that `f(y) = g(x)`, with the constraint `y ≠ 0`.

9.  **Analyze the Functions `f(y)` and `g(x)`:**
    *   `f(y) = y / sinh(y)`:
        *   `f(y)` is an even function: `f(-y) = (-y) / sinh(-y) = (-y) / (-sinh(y)) = y / sinh(y) = f(y)`.
        *   As `y -> 0`, `f(y) -> 1`.
        *   As `y -> ±∞`, `sinh(y)` grows exponentially faster than `y`, so `f(y) -> 0`.
        *   The maximum value is `f(0) = 1` (in the limit). For `y ≠ 0`, `|sinh(y)| > |y|`, so `0 < |f(y)| < 1`.
        *   The range of `f(y)` for `y ≠ 0` is `(0, 1)`. (Actually, need to be careful. `y/sinh(y)` can be negative if sinh(y) and y have opposite signs? No, they always have the same sign. Check derivative: `f'(y) = (sinh(y) - y*cosh(y)) / sinh^2(y)`. The numerator is `sinh(y) - y*cosh(y)`. Let `h(y) = sinh(y) - y*cosh(y)`. `h'(y) = cosh(y) - (cosh(y) + y*sinh(y)) = -y*sinh(y)`. Since `y` and `sinh(y)` always have the same sign, `y*sinh(y) >= 0`. So `h'(y) <= 0`. Since `h(0)=0`, `h(y) < 0` for `y > 0` and `h(y) > 0` for `y < 0`. This means `f'(y) < 0` for `y > 0` and `f'(y) > 0` for `y < 0`. The function decreases from 1 towards 0 as `|y|` increases from 0). The range is indeed `(0, 1)`.

    *   `g(x) = -x * cosh(x)`:
        *   `g(x)` is an odd function: `g(-x) = -(-x) * cosh(-x) = x * cosh(x) = -g(x)`.
        *   `g(0) = 0`.
        *   As `x -> +∞`, `g(x) -> -∞`.
        *   As `x -> -∞`, `g(x) -> +∞`.
        *   The range of `g(x)` is `(-∞, +∞)`.

10. **Combine the Analyses:**
    *   We need to solve `f(y) = g(x)`, where `f(y) = y / sinh(y)` and `g(x) = -x * cosh(x)`.
    *   We know the range of `f(y)` (for `y ≠ 0`) is `(0, 1)`.
    *   We need to find values of `x` for which `g(x)` falls within the range `(0, 1)`.
    *   We need `0 < -x * cosh(x) < 1`.
    *   Since `cosh(x) >= 1` (and strictly positive), for `-x * cosh(x)` to be positive, `x` must be negative. Let `x = -a` where `a > 0`.
    *   The condition becomes `0 < -(-a) * cosh(-a) < 1`
    *   `0 < a * cosh(a) < 1` (where `a = -x > 0`)
    *   Let `h(a) = a * cosh(a)`. `h(0) = 0`. `h'(a) = 1*cosh(a) + a*sinh(a)`. Since `a > 0`, `cosh(a) >= 1` and `sinh(a) > 0`, so `h'(a) > 0`. `h(a)` is strictly increasing for `a > 0`.
    *   We need to find the value of `a > 0` such that `a * cosh(a) = 1`. This equation `a * cosh(a) = 1` needs to be solved numerically. Let's approximate.
        *   If `a = 0.5`, `0.5 * cosh(0.5) ≈ 0.5 * 1.1276 ≈ 0.56 < 1`.
        *   If `a = 1`, `1 * cosh(1) ≈ 1 * 1.543 ≈ 1.54 > 1`.
        *   If `a = 0.8`, `0.8 * cosh(0.8) ≈ 0.8 * 1.337 ≈ 1.07 > 1`.
        *   If `a = 0.7`, `0.7 * cosh(0.7) ≈ 0.7 * 1.255 ≈ 0.878 < 1`.
        *   If `a = 0.75`, `0.75 * cosh(0.75) ≈ 0.75 * 1.294 ≈ 0.97 < 1`.
        *   If `a = 0.77`, `0.77 * cosh(0.77) ≈ 0.77 * 1.313 ≈ 1.01 > 1`.
        *   So, the solution `a_0` for `a * cosh(a) = 1` is approximately `0.76`.
    *   The condition `0 < a * cosh(a) < 1` holds for `0 < a < a_0 ≈ 0.76`.
    *   Since `x = -a`, this means the condition holds for `-a_0 < x < 0` (approximately `-0.76 < x < 0`).

11. **Existence of Solutions:**
    *   For any `x` in the interval `(-a_0, 0)`, the value `g(x) = -x * cosh(x)` lies in the interval `(0, 1)`.
    *   Since the range of `f(y) = y / sinh(y)` (for `y ≠ 0`) is also `(0, 1)`, and `f(y)` is continuous and decreases from 1 to 0 as `|y|` goes from 0 to infinity, for any value `C` in `(0, 1)`, there exist exactly two non-zero values of `y` such that `f(y) = C` (one positive, one negative, since `f(y)` is even).
    *   Therefore, for each `x` in `(-a_0, 0)`, there are exactly two values of `y` (one positive, one negative) that satisfy the equation `y / sinh(y) = -x * cosh(x)`.

12. **Summary of Findings:**
    *   The original equation is `x + y / (cosh(x) * sinh(y)) = 0`.
    *   Requires `y ≠ 0`.
    *   Can be rearranged to `y / sinh(y) = -x * cosh(x)`.
    *   No simple explicit solution for `x` or `y`.
    *   Solutions exist only if `0 < -x * cosh(x) < 1`.
    *   This requires `x` to be negative. Let `a = -x`, so `a > 0`. The condition is `0 < a * cosh(a) < 1`.
    *   The function `a * cosh(a)` increases from 0 for `a > 0`. Let `a_0` be the unique positive solution to `a * cosh(a) = 1` (`a_0 ≈ 0.76`).
    *   Solutions exist if and only if `0 < a < a_0`, which means `-a_0 < x < 0`.
    *   For each `x` in this interval, there are exactly two corresponding values of `y` (symmetric, `y` and `-y`) that satisfy the equation.
    *   There are no solutions if `x >= 0` or `x <= -a_0`.

13. **Final Answer Formulation:**
    *   State the original equation.
    *   State the constraint `y ≠ 0`.
    *   Show the rearrangement `y = -x * cosh(x) * sinh(y)` or `y / sinh(y) = -x * cosh(x)`.
    *   Explain that it's an implicit equation with no simple explicit solution.
    *   Analyze the existence of solutions based on the ranges of `y/sinh(y)` and `-x*cosh(x)`.
    *   Conclude that solutions exist only for `x` in a specific negative interval (`-a_0 < x < 0` where `a_0` solves `a_0 cosh(a_0) = 1`) and for each such `x`, there are two `y` values.
    *   Mention the specific case `x=0` leads to no solution.
    *   It might be useful to plot `y/sinh(y)` and `-x*cosh(x)` to visualize the intersection.