Okay, let's analyze the equation:
`x + y / (cosh(x) * sinh(y)) = 0`

1.  **Identify Constraints:**
    The equation involves division. The denominator `cosh(x) * sinh(y)` cannot be zero.
    *   `cosh(x) = (e^x + e^-x) / 2` is always greater than or equal to 1 for real `x`. It is never zero.
    *   `sinh(y) = (e^y - e^-y) / 2` is zero only when `y = 0`.
    Therefore, the equation is only defined if `sinh(y) ≠ 0`, which means **`y ≠ 0`**.

2.  **Rearrange the Equation:**
    Assuming `y ≠ 0`, we can manipulate the equation:
    `y / (cosh(x) * sinh(y)) = -x`
    Multiply both sides by `cosh(x) * sinh(y)`:
    `y = -x * cosh(x) * sinh(y)`

3.  **Analyze the Rearranged Equation:**
    `y = -x * cosh(x) * sinh(y)`
    This is an **implicit equation**. It defines a relationship between `x` and `y`, but it's generally not possible to isolate `y` explicitly as a function of `x` (`y = f(x)`) or `x` explicitly as a function of `y` (`x = g(y)`) using standard elementary functions.

4.  **Further Rearrangement (Alternative Form):**
    We can also rearrange it slightly differently (still assuming `y ≠ 0`):
    Divide both sides by `sinh(y)`:
    `y / sinh(y) = -x * cosh(x)`

5.  **Existence of Solutions:**
    Let `f(y) = y / sinh(y)` and `g(x) = -x * cosh(x)`. We are looking for pairs `(x, y)` such that `f(y) = g(x)` and `y ≠ 0`.
    *   **Analyze `f(y) = y / sinh(y)`:**
        *   As `y` approaches 0, `sinh(y)` approaches `y`, so `f(y)` approaches 1.
        *   `f(y)` is an even function (`f(-y) = f(y)`).
        *   For any `y ≠ 0`, `|sinh(y)| > |y|`, and `y` and `sinh(y)` always have the same sign. Therefore, `0 < y / sinh(y) < 1`.
        *   The range of `f(y)` for `y ≠ 0` is the interval `(0, 1)`.
    *   **Analyze `g(x) = -x * cosh(x)`:**
        *   `g(0) = 0`.
        *   `cosh(x)` is always positive (≥ 1).
        *   If `x > 0`, `g(x)` is negative.
        *   If `x < 0`, `g(x)` is positive.
        *   The range of `g(x)` is `(-∞, +∞)`.

    *   **Finding Intersections:** We need `f(y) = g(x)`. Since the range of `f(y)` is `(0, 1)`, we must have `0 < g(x) < 1`.
        *   `g(x) > 0` requires `x < 0`.
        *   We need `-x * cosh(x) < 1`. Let `a = -x`, so `a > 0`. The condition becomes `a * cosh(a) < 1`.
        *   The function `h(a) = a * cosh(a)` starts at `h(0)=0` and increases for `a > 0`. There is a unique positive value `a_0` such that `a_0 * cosh(a_0) = 1`. Numerically, `a_0 ≈ 0.76`.
        *   So, the condition `0 < a * cosh(a) < 1` holds for `0 < a < a_0`.
        *   Since `x = -a`, this means solutions can only exist for `x` in the interval `-a_0 < x < 0` (approximately `-0.76 < x < 0`).

    *   **Conclusion on Solutions:**
        *   If `x ≥ 0`, then `g(x) = -x * cosh(x) ≤ 0`. Since `f(y) = y / sinh(y)` is always in `(0, 1)`, there are **no solutions** for `x ≥ 0`.
        *   If `x ≤ -a_0 ≈ -0.76`, then `g(x) = -x * cosh(x) ≥ 1`. Since `f(y)` is always less than 1, there are **no solutions** for `x ≤ -a_0`.
        *   If `-a_0 < x < 0`, then `0 < g(x) < 1`. For any value `C` in `(0, 1)`, the equation `y / sinh(y) = C` has exactly two solutions for `y` (one positive, one negative, symmetric around 0). Therefore, for each `x` in this interval, there are **exactly two values of `y`** that satisfy the original equation.

**Summary:**

The equation `x + y / (cosh(x) * sinh(y)) = 0` implicitly defines a relationship between `x` and `y`.

1.  There is a constraint: **`y ≠ 0`**.
2.  The equation can be written as **`y = -x * cosh(x) * sinh(y)`** or **`y / sinh(y) = -x * cosh(x)`**.
3.  There is **no general explicit solution** for `y` in terms of `x` or vice-versa using elementary functions.
4.  Solutions **only exist** for `x` values in a specific negative interval approximately **`-0.76 < x < 0`**.
5.  For each `x` in this interval, there are **two corresponding `y` values** (one positive, one negative) that satisfy the equation. There are no solutions for `x ≥ 0` or `x ≤ -0.76` (approximately).